revised many definitions to account for exceptions in SABLE C source, now getting back to the correspondence proofs...

Proofs/TPM_Corres.thy
@@ -6,38 +6,21 @@ imports
   "../lib/WP_Extras"
 begin
 
-context sable_verified
+context sable_verified_pp
 begin
 
-abbreviation "PO \<equiv> powerOn \<circ> machine"
-abbreviation "PO' \<equiv> powerOn \<circ> phantom_machine_state_''"
-abbreviation "corres \<equiv> \<lambda>rrel G G'. corres_underlying R False True rrel
-                (\<lambda>s. PO s \<and> G s) (\<lambda>s'. PO' s' \<and> G' s')"
-abbreviation "corres_off \<equiv> \<lambda>rrel G G'. corres_underlying R False True rrel
-                (\<lambda>s. \<not>PO s \<and> G s) (\<lambda>s'. \<not>PO' s' \<and> G' s')"
-
-lemma corres_off_valid: "\<And>rrel G G' m m'. corres_off rrel G G' m m'"
-unfolding R_def corres_underlying_def by auto
-
-(* FIXME: reason about size, value *)
-definition
-  StoredData_rel :: "string TPM.STORED_DATA \<Rightarrow> (8 word ptr \<times> 32 word) \<times> lifted_globals \<Rightarrow> bool"
-where
-  "StoredData_rel d d' \<equiv> case d' of ((v', size'), s') \<Rightarrow>
-    \<forall>p \<in> fst (unpack_TPM_STORED_DATA12' v' size' s'). STORED_DATA_rel \<top>\<top> d p"
+abbreviation "corres \<equiv> corres_underlying R False True"
 
 end
 
-locale sable_m = sable_verified +
-  assumes get_authdata_corres: "corres (\<lambda>r r'. AUTHDATA_rel r (fst r'))
+locale sable_m = sable_verified_pp +
+  assumes get_authdata_corres: "corres (\<lambda>r r'. R_AUTHDATA_rel r (fst r'))
                                   \<top> \<top> get_authdata get_authdata'"
 
-      and get_nonce_corres: "corres (\<lambda>r r'. NONCE_rel r (fst r')) \<top> \<top> get_nonce get_nonce'"
-
-      and exit_corres: "\<And>P P'. corres \<top>\<top> P P' exit exit'"
+      and get_nonce_corres: "corres (\<lambda>r r'. R_NONCE_rel r (fst r')) \<top> \<top> get_nonce get_nonce'"
 
       and TPM_PCRRead_corres: "\<And>i i'. PCRINDEX_rel i i' \<Longrightarrow>
-        corres (\<lambda>r r'. TPM_PCRRead_rel r (fst r')) \<top> \<top> (TPM_PCRRead i) (TPM_PCRRead' i')"
+        corres (\<lambda>r r'. R_PCRVALUE_rel r (fst r')) \<top> \<top> (TPM_PCRRead i) (TPM_PCRRead' i')"
 
       and TPM_OIAP_corres: "\<And>sess'. corres (\<lambda>r r'. RESULT_rel r (fst r'))
           \<top> (\<lambda>s'. is_valid_tdTPM_SESSION_C'ptr s' sess') TPM_OIAP (TPM_OIAP' sess')"
@@ -45,18 +28,7 @@ locale sable_m = sable_verified +
       (* FIXME: add constraints to the authdata/session inputs *)
       and TPM_NV_ReadValue_corres: "\<And>P P' idx idx' off off' a size' ownerAuth' s'.
         \<lbrakk>idx' = of_nat idx; off' = of_nat off\<rbrakk>
-        \<Longrightarrow> corres (TPM_NV_ReadValue_rel StoredData_rel) P P' (TPM_NV_ReadValue idx off a)
-        (TPM_NV_ReadValue' idx' off' size' ownerAuth' s')"
-
-context sable_m
-begin
-
-lemma exit: "\<lbrace>\<top>\<rbrace> exit \<lbrace>\<lambda>_ s. \<not>PO s\<rbrace>"
-unfolding exit_def by (wp, auto)
-
-lemma exit': "\<lbrace>\<top>\<rbrace> exit' \<lbrace>\<lambda>_ s'. \<not>PO' s'\<rbrace>"
-using exit_corres
-
-end
+        \<Longrightarrow> corres (R_HEAP_DATA_rel (E_STORED_DATA_rel string_rel)) P P'
+        (TPM_NV_ReadValue idx off a) (TPM_NV_ReadValue' idx' off' size' ownerAuth' s')"
 
 end
